common/Memory.v
@@ -40,6 +40,7 @@ Require Import Values.
 Require Import Tags.
 Require Import Memdata.
 Require Import Builtins.
+Require Import Encoding.
 Require Import ExtLib.Structures.Monads. Import MonadNotation.
 Global Open Scope monad_scope.
 
@@ -81,11 +82,19 @@ Module Type Memory (Ptr: Pointer) (Pol:Policy).
   Import TLib.
   Export Ptr.
 
+  Parameter addr : Type.
+  Parameter of_ptr : ptr -> addr.
+  Parameter addr_off : addr -> int64 -> addr.
+
+  (*Parameter addr_off_distributes :
+    forall p ofs,
+      of_ptr (off p ofs) = addr_off (of_ptr p) ofs.*)
+  
   Parameter mem : Type.
   
   (** Permissions *)
-  Parameter allowed_access : mem -> memory_chunk -> ptr -> Prop.
-  Parameter aligned_access : memory_chunk -> ptr -> Prop.
+  Parameter allowed_access : mem -> memory_chunk -> addr -> Prop.
+  Parameter aligned_access : memory_chunk -> addr -> Prop.
   
   Parameter allowed_access_dec:
     forall m chunk a,
@@ -107,11 +116,11 @@ Module Type Memory (Ptr: Pointer) (Pol:Policy).
       [a].  It returns the value of the memory chunk
       at that address.  [None] is returned if the accessed bytes
       are not readable. *)
-  Parameter load : memory_chunk -> mem -> ptr -> MemoryResult atom.
+  Parameter load : memory_chunk -> mem -> addr -> MemoryResult atom.
 
-  Parameter load_ltags : memory_chunk -> mem -> ptr -> MemoryResult (list tag).
+  Parameter load_ltags : memory_chunk -> mem -> addr -> MemoryResult (list tag).
 
-  Parameter load_all : memory_chunk -> mem -> ptr -> MemoryResult (atom * list tag).
+  Parameter load_all : memory_chunk -> mem -> addr -> MemoryResult (atom * list tag).
   
   Parameter load_all_compose :
     forall chunk m a v lts,
@@ -127,9 +136,9 @@ Module Type Memory (Ptr: Pointer) (Pol:Policy).
       location [(b, ofs)].  Returns [None] if the accessed locations are
       not readable. *)
 
-  Parameter loadbytes : mem -> ptr -> Z -> MemoryResult (list memval).
+  Parameter loadbytes : mem -> addr -> Z -> MemoryResult (list memval).
 
-  Parameter loadtags : mem -> ptr -> Z -> MemoryResult (list tag).
+  Parameter loadtags : mem -> addr -> Z -> MemoryResult (list tag).
 
   (** Memory stores. *)
   
@@ -138,20 +147,20 @@ Module Type Memory (Ptr: Pointer) (Pol:Policy).
       Return the updated memory store, or [None] if the accessed bytes
       are not writable. *)
   
-  Parameter store : memory_chunk -> mem -> ptr -> atom -> list tag -> MemoryResult mem.
+  Parameter store : memory_chunk -> mem -> addr -> atom -> list tag -> MemoryResult mem.
 
-  Parameter store_atom : memory_chunk -> mem -> ptr -> atom -> MemoryResult mem.
+  Parameter store_atom : memory_chunk -> mem -> addr -> atom -> MemoryResult mem.
   
   (** [storebytes m ofs bytes] stores the given list of bytes [bytes]
       starting at location [(b, ofs)].  Returns updated memory state
       or [None] if the accessed locations are not writable. *)
-  Parameter storebytes : mem -> ptr -> list memval -> list tag -> MemoryResult mem.
+  Parameter storebytes : mem -> addr -> list memval -> list tag -> MemoryResult mem.
   
   Global Opaque Memory.store Memory.load Memory.storebytes Memory.loadbytes.
 
 End Memory.
 
-Module ConcMem (Ptr: Pointer) (Pol:Policy).
+Module ConcMem (Ptr: Pointer) (Pol:Policy) <: Memory Ptr Pol.
   Module BI := Builtins Ptr.
   Export BI.
   Module MD := Memdata Ptr Pol.
@@ -159,47 +168,213 @@ Module ConcMem (Ptr: Pointer) (Pol:Policy).
   Import TLib.
   Export Ptr.
 
-  Parameter mem : Type.
+  Inductive permission : Type := Live | Dead | MostlyDead.
+
+  Lemma permission_dec : forall (p1 p2 : permission), {p1 = p2} + {p1 <> p2}.
+  Proof.
+    intros. destruct p1; destruct p2; try (right; intro; discriminate); left; auto.
+  Qed.
+
+  Definition addr : Type := int64.
+  Definition of_ptr (p: ptr) : addr := concretize p.
+
+  Definition addr_off (a: addr) (i: int64) : addr :=
+    Int64.add a i.
   
-  Parameter allowed_access : mem -> memory_chunk -> ptr -> Prop.
-  Parameter aligned_access : memory_chunk -> ptr -> Prop.
+  Record mem' : Type := mkmem {
+    mem_contents: ZMap.t (memval*tag);  (**r [offset -> memval] *)
+    mem_access: ZMap.t permission;      (**r [offset -> kind -> option permission] *)
+    live: list (Z*Z);
+  }.
+
+  Definition mem : Type := mem'.
   
-  Parameter allowed_access_dec:
+  Definition get_perm (m: mem) (a: addr) : permission :=
+    ZMap.get (Int64.unsigned a) m.(mem_access).
+  
+  Definition perm (m: mem) (a: addr) (p: permission) : Prop :=
+    get_perm m a = p.
+
+  Theorem perm_dec:
+    forall m ofs p, {perm m ofs p} + {~ perm m ofs p}.
+  Proof.
+    unfold perm; intros. eapply permission_dec.
+  Defined.
+
+  Definition range_perm (m: mem) (lo hi: Z) (p: permission) : Prop :=
+    forall a, lo <= a < hi -> perm m (Int64.repr a) p.
+
+  Lemma range_perm_dec:
+    forall m lo hi p, {range_perm m lo hi p} + {~ range_perm m lo hi p}.
+  Proof.
+    intros.
+    induction lo using (well_founded_induction_type (Zwf_up_well_founded hi)).
+    destruct (zlt lo hi) eqn:?.
+    - destruct (perm_dec m (Int64.repr lo) p).
+      + destruct (H (lo + 1)).
+        * red. lia.
+        * left; red; intros. destruct (zeq lo a).
+          -- rewrite e in p0. congruence.
+          -- apply r. lia.
+        * right; red; intros. elim n. red; intros; apply H0; lia.
+      + right; red; intros. elim n. apply H0.
+        lia.
+    - left; red; intros. extlia.
+  Defined.
+  
+  Definition range_perm_neg (m: mem) (lo hi: Z) (p: permission) : Prop :=
+    forall a, lo <= a < hi -> ~ perm m (Int64.repr a) p.
+  (** * Operations over memory stores *)
+ 
+  Lemma range_perm_neg_dec:
+    forall m lo hi p, {range_perm_neg m lo hi p} + {~ range_perm_neg m lo hi p}.
+  Proof.
+    intros.
+    induction lo using (well_founded_induction_type (Zwf_up_well_founded hi)).
+    destruct (zlt lo hi).
+    - destruct (perm_dec m (Int64.repr lo) p).
+      + right; red; intros. apply (H0 lo). lia. auto.
+      + destruct (H (lo + 1)).
+        * red. lia.
+        * left; red; intros. destruct (zeq lo a).
+          -- congruence.
+          -- apply r. lia.
+        * right; red; intros. elim n0. red; intros. apply H0; lia.
+    - left; red; intros. extlia.
+  Defined.
+
+  Definition allowed_access (m: mem) (chunk: memory_chunk) (a: addr) : Prop :=
+    range_perm_neg m (Int64.unsigned a) ((Int64.unsigned a) + size_chunk chunk) Dead.
+
+  Definition aligned_access (chunk: memory_chunk) (a: addr) : Prop :=
+    (align_chunk chunk | (Int64.unsigned a)).
+
+  Lemma allowed_access_dec:
     forall m chunk a,
       {allowed_access m chunk a} + {~ allowed_access m chunk a}.
+  Proof.
+    intros.
+    destruct (range_perm_neg_dec m (Int64.unsigned a) ((Int64.unsigned a) + size_chunk chunk) Dead).
+    left; auto.
+    right; red; contradiction.
+  Defined.
 
-  Parameter aligned_access_dec:
+  Lemma aligned_access_dec:
     forall chunk a,
       {aligned_access chunk a} + {~ aligned_access chunk a}.
+  Proof.
+    intros. destruct (Zdivide_dec (align_chunk chunk) (Int64.unsigned a)); auto.
+  Qed.
+
+  Definition empty: mem :=
+    mkmem (ZMap.init (Undef, def_tag))
+          (ZMap.init MostlyDead)
+          [].
+
+  Fixpoint getN (n: nat) (p: Z) (c: ZMap.t (memval*tag)) {struct n}: list (memval * tag) :=
+    match n with
+    | O => nil
+    | S n' => ZMap.get p c :: getN n' (p + 1) c
+    end.
   
-  Parameter empty : mem.
+  Definition load (chunk: memory_chunk) (m: mem) (a: addr): MemoryResult atom :=
+    if aligned_access_dec chunk a then
+      if allowed_access_dec m chunk a
+      then MemorySuccess (decode_val chunk (map (fun x => fst x) (getN (size_chunk_nat chunk) (Int64.unsigned a) (m.(mem_contents)))))
+      else MemoryFail "" (PrivateLoad (Int64.unsigned a))
+    else MemoryFail "" (MisalignedLoad (align_chunk chunk) (Int64.unsigned a)).
 
-  Parameter load : memory_chunk -> mem -> ptr -> MemoryResult atom.
+  Definition load_ltags (chunk: memory_chunk) (m: mem) (a: addr): MemoryResult (list tag) :=
+    if aligned_access_dec chunk a then
+      if allowed_access_dec m chunk a
+      then MemorySuccess (map (fun x => snd x) (getN (size_chunk_nat chunk) (Int64.unsigned a) (m.(mem_contents))))
+      else MemoryFail "" (PrivateLoad (Int64.unsigned a))
+    else MemoryFail "" (MisalignedLoad (align_chunk chunk) (Int64.unsigned a)).
 
-  Parameter load_ltags : memory_chunk -> mem -> ptr -> MemoryResult (list tag).
-
-  Parameter load_all : memory_chunk -> mem -> ptr -> MemoryResult (atom * list tag).
+Definition load_all (chunk: memory_chunk) (m: mem) (a: addr): MemoryResult (atom * list tag) :=
+    if aligned_access_dec chunk a then
+      if allowed_access_dec m chunk a
+      then MemorySuccess (decode_val chunk
+                                     (map (fun x => fst x)
+                                          (getN (size_chunk_nat chunk)
+                                                (Int64.unsigned a) (m.(mem_contents)))),
+                           map (fun x => snd x) (getN (size_chunk_nat chunk) (Int64.unsigned a) (m.(mem_contents))))
+      else MemoryFail "" (PrivateLoad (Int64.unsigned a))
+    else MemoryFail "" (MisalignedLoad (align_chunk chunk) (Int64.unsigned a)).
   
-  Parameter load_all_compose :
+  Lemma load_all_compose :
     forall chunk m a v lts,
       load_all chunk m a = MemorySuccess (v,lts) <->
         load chunk m a = MemorySuccess v /\ load_ltags chunk m a = MemorySuccess lts.
+  Proof.
+    intros until lts.
+    unfold load_all; unfold load; unfold load_ltags.
+    split.
+    - destruct (aligned_access_dec chunk a); destruct (allowed_access_dec m chunk a); intro H; inv H; auto.
+    - destruct (aligned_access_dec chunk a); destruct (allowed_access_dec m chunk a); intro H; destruct H as [H1 H2]; inv H1; inv H2; auto.
+  Qed.
 
-  Parameter load_all_fail :
+  Lemma load_all_fail :
     forall chunk m a msg failure,
       load_all chunk m a = MemoryFail msg failure <->
         load chunk m a = MemoryFail msg failure /\ load_ltags chunk m a = MemoryFail msg failure.
+  Proof.
+    intros until failure.
+    unfold load_all; unfold load; unfold load_ltags.
+    split.
+    - destruct (aligned_access_dec chunk a); destruct (allowed_access_dec m chunk a); intro H; inv H; auto.
+    - destruct (aligned_access_dec chunk a); destruct (allowed_access_dec m chunk a); intro H; destruct H as [H1 H2]; inv H1; inv H2; auto.
+  Qed. 
+
+  Definition loadbytes (m: mem) (a: addr) (n: Z): MemoryResult (list memval) :=
+    if range_perm_neg_dec m (Int64.unsigned a) ((Int64.unsigned a) + n) Dead
+    then MemorySuccess (map (fun x => fst x) (getN (Z.to_nat n) (Int64.unsigned a) (m.(mem_contents))))
+    else MemoryFail "" (PrivateLoad (Int64.unsigned a)).
+
+  Definition loadtags (m: mem) (a: addr) (n: Z) : MemoryResult (list tag) :=
+    if range_perm_neg_dec m (Int64.unsigned a) ((Int64.unsigned a) + n) Dead
+    then MemorySuccess (map (fun x => snd x) (getN (Z.to_nat n) (Int64.unsigned a) (m.(mem_contents))))
+    else MemoryFail "" (PrivateLoad (Int64.unsigned a)).
+
+  Fixpoint setN (vl: list (memval*tag)) (p: Z) (c: ZMap.t (memval*tag)) {struct vl}: ZMap.t (memval*tag) :=
+    match vl with
+    | nil => c
+    | v :: vl' => setN vl' (p + 1) (ZMap.set p v c)
+    end.
+
+  Fixpoint merge_vals_tags (vs:list memval) (lts:list tag) :=
+    match vs with
+    | v::vs' =>
+        (v,hd def_tag lts)::(merge_vals_tags vs' (tl lts))
+    | _ => []
+    end.
   
-  Parameter loadbytes : mem -> ptr -> Z -> MemoryResult (list memval).
+  Definition store (chunk: memory_chunk) (m: mem) (a: addr) (v:atom) (lts:list tag)
+    : MemoryResult mem :=
+    if aligned_access_dec chunk a then
+      if allowed_access_dec m chunk a then
+        MemorySuccess (mkmem (setN (merge_vals_tags (encode_val chunk v) lts) (Int64.unsigned a) (m.(mem_contents)))
+                             m.(mem_access) m.(live))
+      else MemoryFail "" (PrivateStore (Int64.unsigned a))
+    else MemoryFail "" (MisalignedStore (align_chunk chunk) (Int64.unsigned a)).
 
-  Parameter loadtags : mem -> ptr -> Z -> MemoryResult (list tag).
+  Definition store_atom (chunk: memory_chunk) (m: mem) (a: addr) (v: atom)
+    : MemoryResult mem :=
+    if aligned_access_dec chunk a then
+      if allowed_access_dec m chunk a then
+        let lts := map snd (getN (Z.to_nat (size_chunk chunk)) (Int64.unsigned a) (m.(mem_contents))) in
+        MemorySuccess (mkmem (setN (merge_vals_tags (encode_val chunk v) lts) (Int64.unsigned a) (m.(mem_contents)))
+                             m.(mem_access) m.(live))
+      else MemoryFail "" (PrivateStore (Int64.unsigned a))
+    else MemoryFail "" (MisalignedStore (align_chunk chunk) (Int64.unsigned a)).
 
-  Parameter store : memory_chunk -> mem -> ptr -> atom -> list tag ->
-                    MemoryResult mem.
-
-  Parameter store_atom : memory_chunk -> mem -> ptr -> atom -> MemoryResult mem.
-  
-  Parameter storebytes : mem -> ptr -> list memval -> list tag -> MemoryResult mem.
+  Definition storebytes (m: mem) (a: addr) (bytes: list memval) (lts:list tag)
+    : MemoryResult mem :=
+    if range_perm_neg_dec m (Int64.unsigned a) ((Int64.unsigned a) + Z.of_nat (length bytes)) Dead then
+      MemorySuccess (mkmem
+                       (setN (merge_vals_tags bytes lts) (Int64.unsigned a) (m.(mem_contents)))
+                       m.(mem_access) m.(live))
+    else MemoryFail "" (PrivateStore (Int64.unsigned a)).
   
 End ConcMem.
 
@@ -213,6 +388,11 @@ Module MultiMem (Pol: Policy) : Memory SemiconcretePointer Pol.
   Export TLib.
   Export SemiconcretePointer.
 
+  Definition addr : Type := ptr.
+  Definition of_ptr (p: ptr) : addr := p.
+
+  Definition addr_off := off.
+  
   Record myMem := mkMem
     {
       comp_locals : PMap.t CM.mem;
@@ -221,13 +401,13 @@ Module MultiMem (Pol: Policy) : Memory SemiconcretePointer Pol.
   
   Definition mem : Type := myMem.
   
-  Definition allowed_access (m: mem) (chunk: memory_chunk) (p: ptr) : Prop :=
-    match p with
-    | (LocInd C, i) => CM.allowed_access (m.(comp_locals)#C) chunk p
-    | (ShareInd b _, i) => CM.allowed_access (m.(comp_locals)#b) chunk p
+  Definition allowed_access (m: mem) (chunk: memory_chunk) (a: addr) : Prop :=
+    match a with
+    | (LocInd C, i) => CM.allowed_access (m.(comp_locals)#C) chunk i
+    | (ShareInd b _, i) => CM.allowed_access (m.(comp_locals)#b) chunk i
     end.
     
-  Parameter aligned_access : memory_chunk -> ptr -> Prop.
+  Parameter aligned_access : memory_chunk -> addr -> Prop.
   
   Parameter allowed_access_dec:
     forall m chunk a,
@@ -240,22 +420,22 @@ Module MultiMem (Pol: Policy) : Memory SemiconcretePointer Pol.
   Definition empty : mem :=
     mkMem (PMap.init CM.empty) (PMap.init CM.empty).
   
-  Definition load (chunk: memory_chunk) (m: mem) (p: ptr) : MemoryResult atom :=
-    match p with
-    | (LocInd C, i) => CM.load chunk (m.(comp_locals)#C) p
-    | (ShareInd b _, i) => CM.load chunk (m.(comp_locals)#b) p
+  Definition load (chunk: memory_chunk) (m: mem) (a: addr) : MemoryResult atom :=
+    match a with
+    | (LocInd C, i) => CM.load chunk (m.(comp_locals)#C) i
+    | (ShareInd b _, i) => CM.load chunk (m.(comp_locals)#b) i
     end.
 
-  Definition load_ltags (chunk: memory_chunk) (m: mem) (p: ptr) : MemoryResult (list tag) :=
-    match p with
-    | (LocInd C, i) => CM.load_ltags chunk (m.(comp_locals)#C) p
-    | (ShareInd b _, i) => CM.load_ltags chunk (m.(comp_locals)#b) p
+  Definition load_ltags (chunk: memory_chunk) (m: mem) (a: addr) : MemoryResult (list tag) :=
+    match a with
+    | (LocInd C, i) => CM.load_ltags chunk (m.(comp_locals)#C) i
+    | (ShareInd b _, i) => CM.load_ltags chunk (m.(comp_locals)#b) i
     end.
   
-  Definition load_all (chunk: memory_chunk) (m: mem) (p: ptr) : MemoryResult (atom * list tag) :=
-    match p with
-    | (LocInd C, i) => CM.load_all chunk (m.(comp_locals)#C) p
-    | (ShareInd b _, i) => CM.load_all chunk (m.(comp_locals)#b) p
+  Definition load_all (chunk: memory_chunk) (m: mem) (a: addr) : MemoryResult (atom * list tag) :=
+    match a with
+    | (LocInd C, i) => CM.load_all chunk (m.(comp_locals)#C) i
+    | (ShareInd b _, i) => CM.load_all chunk (m.(comp_locals)#b) i
     end.
   
   Lemma load_all_compose :
@@ -276,50 +456,49 @@ Module MultiMem (Pol: Policy) : Memory SemiconcretePointer Pol.
     destruct a; destruct i; apply CM.load_all_fail.
   Qed.
   
-  Definition loadbytes (m: mem) (p: ptr) (num: Z) : MemoryResult (list memval) :=
-    match p with
-    | (LocInd C, i) => CM.loadbytes (m.(comp_locals)#C) p num
-    | (ShareInd b _, i) => CM.loadbytes (m.(comp_locals)#b) p num
+  Definition loadbytes (m: mem) (a: addr) (num: Z) : MemoryResult (list memval) :=
+    match a with
+    | (LocInd C, i) => CM.loadbytes (m.(comp_locals)#C) i num
+    | (ShareInd b _, i) => CM.loadbytes (m.(comp_locals)#b) i num
     end.    
 
-  Definition loadtags (m: mem) (p: ptr) (num: Z) : MemoryResult (list tag) :=
-    match p with
-    | (LocInd C, i) => CM.loadtags (m.(comp_locals)#C) p num
-    | (ShareInd b _, i) => CM.loadtags (m.(comp_locals)#b) p num
+  Definition loadtags (m: mem) (a: addr) (num: Z) : MemoryResult (list tag) :=
+    match a with
+    | (LocInd C, i) => CM.loadtags (m.(comp_locals)#C) i num
+    | (ShareInd b _, i) => CM.loadtags (m.(comp_locals)#b) i num
     end.    
 
-  Definition store (chunk: memory_chunk) (m: mem) (p: ptr) (v: atom) (lts: list tag)
+  Definition store (chunk: memory_chunk) (m: mem) (a: addr) (v: atom) (lts: list tag)
     : MemoryResult mem :=
-    match p with
+    match a with
     | (LocInd C, i) =>
-        cm <- CM.store chunk (m.(comp_locals)#C) p v lts;;
+        cm <- CM.store chunk (m.(comp_locals)#C) i v lts;;
         ret (mkMem (PMap.set C cm m.(comp_locals)) m.(shares))
     | (ShareInd b _, i) =>
-        cm <- CM.store chunk (m.(shares)#b) p v lts;;
+        cm <- CM.store chunk (m.(shares)#b) i v lts;;
         ret (mkMem (PMap.set b cm m.(shares)) m.(comp_locals))
     end.
     
-  Definition store_atom (chunk: memory_chunk) (m: mem) (p: ptr) (v: atom)
+  Definition store_atom (chunk: memory_chunk) (m: mem) (a: addr) (v: atom)
     : MemoryResult mem :=
-    match p with
+    match a with
     | (LocInd C, i) =>
-        cm <- CM.store_atom chunk (m.(comp_locals)#C) p v;;
+        cm <- CM.store_atom chunk (m.(comp_locals)#C) i v;;
         ret (mkMem (PMap.set C cm m.(comp_locals)) m.(shares))
     | (ShareInd b _, i) =>
-        cm <- CM.store_atom chunk (m.(shares)#b) p v;;
+        cm <- CM.store_atom chunk (m.(shares)#b) i v;;
         ret (mkMem (PMap.set b cm m.(shares)) m.(comp_locals))
     end.
-  
+
   Definition storebytes (m: mem) (p: ptr) (mvs: list memval) (lts: list tag) :
     MemoryResult mem :=
     match p with
     | (LocInd C, i) =>
-        cm <- CM.store_atom chunk (m.(comp_locals)#C) p v;;
+        cm <- CM.storebytes (m.(comp_locals)#C) i mvs lts;;
         ret (mkMem (PMap.set C cm m.(comp_locals)) m.(shares))
     | (ShareInd b _, i) =>
-        cm <- CM.store_atom chunk (m.(shares)#b) p v;;
+        cm <- CM.storebytes (m.(shares)#b) i mvs lts;;
         ret (mkMem (PMap.set b cm m.(shares)) m.(comp_locals))
-    end.
-    
+    end.    
 
 End MultiMem.
